% For page about spherical to cartesian transformations for velocities
\documentclass{article}
\begin{document}
\begin{math}
$$
\dot{X}\ \ \ \dot{Y}\ \ \ \dot{Z}
\\\\
X, Y, Z, \dot{X}, \dot{Y}, \dot{Z}
\\\\
\dot{\rho}, \dot{\theta}, \dot{\varphi},
\\\\
% base equation (formula 1)
\left\lbrace
\begin{array}{l}
X=\rho\cos{\varphi}\cos{\theta}\\
Y=\rho\cos{\varphi}\sin{\theta}\\
Z=\rho\sin{\varphi}\\
\end{array}
\right.
\\\\\\\\
% sphere to cart - positions
\left\lbrace
\begin{array}{l}
\rho = \sqrt{X^2+Y^2+Z^2}\\
\theta=\arcsin{\frac{Y}{X}}\\
\varphi=\arctan{\frac{Z}{\sqrt{X^2+Y^2+Z^2}}}\\
\end{array}
\right.
\\\\\\\\
\left\lbrace
\begin{array}{l}
\rho\in[0, +\infty[\\
\theta\in[0, 2\pi[\\
\varphi\in[-\frac{\pi}{2},\frac{\pi}{2}[\\
\end{array}
\right.
\\\\
%
% derivation (formula 2)
%
\left\lbrace
\begin{array}{l}
\dot{X}=\cos{\varphi}\cos{\theta}\dot{\rho} + \rho\cos{\varphi}\sin{\theta}\dot{\theta} + \rho\sin{\varphi}\cos{\theta}\dot{\varphi}\\
\dot{Y}=\cos{\varphi}\sin{\theta}\dot{\rho} - \rho\cos{\varphi}\cos{\theta}\dot{\theta} + \rho\sin{\varphi}\sin{\theta}\dot{\varphi}\\
\dot{Z}=\sin{\varphi}\dot{\rho} - \rho\cos{\varphi}\dot{\varphi}\\
\end{array}
\right.
%
\Longrightarrow
\left\lbrace
\begin{array}{l}
\dot{X}=\frac{X}{\rho}\dot{\rho} + Y\dot{\theta} + Z\cos{\theta}\dot{\varphi}\\
\dot{Y}=\frac{Y}{\rho}\dot{\rho} - X\dot{\theta} + Z\sin{\theta}\dot{\varphi}\\
\dot{Z}= \frac{Z}{\rho}\dot{\rho} - \rho\cos{\varphi}\dot{\varphi}
\end{array}
\right.
\\\\
%
%Intermediate formulae
%
\rho = \sqrt{X^2+Y^2+Z^2}
\\\\
X^2+Y^2=\rho^2cos^2\varphi \Rightarrow \rho\cos{\varphi}=\sqrt{X^2+Y^2}
\\\\
cos{\theta}=\frac{X}{\rho\cos{\varphi}} \Rightarrow cos{\theta}=\frac{X}{\sqrt{X^2+Y^2}}
\\\\
sin{\theta}=\frac{Y}{\rho\cos{\varphi}} \Rightarrow sin{\theta}=\frac{Y}{\sqrt{X^2+Y^2}}
%
%2nd expression of formula 2
%
\\\\
\left\lbrace
\begin{array}{l}
\dot{X}=\frac{X}{\sqrt{X^2+Y^2+Z^2}}\dot{\rho} + Y\dot{\theta} + \frac{ZX}{\sqrt{X^2+Y^2}}\dot{\varphi}\\\\
\dot{Y}=\frac{Y}{\sqrt{X^2+Y^2+Z^2}}\dot{\rho} - X\dot{\theta} + \frac{ZY}{\sqrt{X^2+Y^2}}\dot{\varphi}\\\\
\dot{Z}= \frac{Z}{\sqrt{X^2+Y^2+Z^2}}\dot{\rho} - \sqrt{X^2+Y^2}\dot{\varphi}\\\\
\end{array}
\right.
%
%Final results
%
\\\\
\\\\
\left\lbrace
\begin{array}{l}
\dot{\rho} = \frac{X\dot{X} + Y\dot{Y} + Z\dot{Z}}{\sqrt{X^2+Y^2+Z^2}}\\\\
\dot{\theta} = \frac{\dot{X}Y - X\dot{Y}}{X^2+Y^2}\\\\
\dot{\varphi} = \frac{Z(X\dot{X}+Y\dot{Y})-(X^2+Y^2)\dot{Z}}{(X^2+Y^2+Z^2)\sqrt{X^2+Y^2}}\\\\
\end{array}
\right.
$$
\end{math}
\end{document}